---
title: "The Lost Cow"
year: "2017"
month: "US Open"
division: "Bronze"
index: 1
---

## Solution 1

```c++
#include <bits/stdc++.h>
#define int long long
#define double long double
#define NL "\n"
using namespace std;
signed main() {
  cin.tie(0)->sync_with_stdio(0);
  freopen("lostcow.in", "r", stdin);
  freopen("lostcow.out", "w", stdout);
  int x, y, count = 0, pointer, delta = 1;
  cin >> x >> y;
  pointer = x;
  while (1) {
    if ((delta > 0 && x < y && x + delta >= y) ||
        (delta < 0 && x > y && x + delta <= y)) {
      count += abs(pointer - y);
      break;
    }
    count += abs(pointer - x - delta);
    pointer = x + delta;
    delta *= -2;
  }
  cout << count << NL;
}
```

## Solution 2

Here is an $ O(1) $ solution. Let's define $ z = |x - y| $ and refer to $ x $ as the "origin".

We can break down the zig-zag process into two parts:

1. Keep zig-zagging, starting and stopping at the origin, until it is possible to go a distance $ z $ to Bessie. This process will be explained in more detail later.
2. Do the final $ z $ steps.

Let's define a function $ f(n) $ as the number of steps it takes to start and end at the origin while turning $ n $ times. The answer for $ f(n) $ will represent the solution for the first part of the zig-zag process. Here are some examples to clarify the function's purpose:

- $ f(0) = 0 $: For the test case $ (x = 3) \rightarrow (y = 4) $, we don't need to take any turns since Farmer John can just walk to $ x + 1 $. We can express the answer to this test case as $ f(0) + |3 - 4| $.

- $ f(1) = 2 $: Given the test case $ (x = 3) \rightarrow (y = 2) $, we need to turn once. Our steps to reach the origin again with one turn are $ 3 \rightarrow 4 \rightarrow 3 $, hence $ f(1) = 2 $. We can express the answer as $ f(1) + |3 - 2| $.

Since for all $ f(n) $, we start and end at the origin, we can base $ f(n) $ on $ f(n - 1) $. For $ f(1) $, we walk forward $ 1 $ step and then backward $ 1 $ step. For $ f(2) $, we walk backward $ 2 $ steps and then forward $ 2 $ steps, in addition to the steps taken for $ f(1) $. For $ f(3) $, we walk forward $ 4 $ steps and then backward $ 4 $ steps, in addition to the steps taken for $ f(2) $.

Here's all the equations:

- $ f(0) = 0 $
- $ f(1) = f(0) + 1 + 1 = f(0) + 2 = f(0) + 2^1 $
- $ f(2) = f(1) + 2 + 2 = f(1) + 4 = f(1) + 2^2 $
- $ f(3) = f(2) + 4 + 4 = f(2) + 8 = f(2) + 2^3 $

Expanding the recursive formula for $ f(3) $:

$$
f(3) = 2^3 + 2^2 + 2^1
$$

Factoring out $ 2 $:

$$
f(3) = 2(2^2 + 2^1 + 2^0)
$$

Noticing that $ 2^2 + 2^1 + 2^0 = 2^3 - 1 $, we get:

$$
f(3) = 2(2^3 - 1)
$$

Generalizing for any $ n $:

$$
f(n) = 2(2^n - 1)
$$

Now that we know this, we have to find the appropriate $ n $ for each test case. We can break this task down into two cases:

1. $ x < y $: $ a = \{1, 4, 16, 64, \ldots\} $ represents the maximum possible distance Farmer John can walk to the right from the origin after $ n = \{0, 2, 4, 6, \ldots\} $ turns (since all other powers of $2$ are for walking to the left). A function that fits this pattern is $ n_i = 2 \times \log_4{(a_i)} $. To generalize this function for all positive integers, we ensure that distances like $ 2 $ and $ 3 $ "round up" to $ 4 $ using a ceiling operation: $ n = 2 \times \lceil \log_4{(z)} \rceil $.

2. $ x > y $: $ a = \{2, 8, 32, 128, \ldots\} $ represents the maximum possible distance Farmer John can walk to the left from the origin after $ n = \{1, 3, 5, 7, \ldots\} $ turns. It's clear that dividing each $ a_i $ by $ 2 $ and applying the function from the first case will result in $ n_i $ being $ 1 $ less than the correct result. Therefore, $ n = 2 \times \lceil \log_4{(z / 2)} \rceil + 1 $.

All together...

```c++
#include <bits/stdc++.h>
#define int long long
#define double long double
#define NL "\n"
using namespace std;
signed main() {
  cin.tie(0)->sync_with_stdio(0);
  freopen("lostcow.in", "r", stdin);
  freopen("lostcow.out", "w", stdout);
  int x, y;
  cin >> x >> y;
  int z = abs(y - x);
  int n = (y > x) ? 2 * ceil(log(z) / log(4.0L))
                  : 2 * ceil(log(z / 2.0L) / log(4.0L)) + 1;
  cout << 2 * ((1LL << n) - 1) + z << NL;
}
```
